Insert Vale poly1305 proofs into EverCrypt.Poly1305

providers/evercrypt/fst/EverCrypt.Poly1305.fst
@@ -28,8 +28,9 @@ let poly1305 dst src len key =
     Poly_stdcalls.poly1305 ctx src (FStar.Int.Cast.Full.uint32_to_uint64 len);
     B.blit ctx 0ul dst 0ul 16ul;
     let h1 = ST.get () in
-    // Missing spec equivalence proof here.
-    assume (B.as_seq h1 dst == Spec.Poly1305.poly1305 (B.as_seq h0 src) (B.as_seq h0 key));
+    X64.Poly1305.CallingFromLowStar.lemma_call_poly1305 h0 h1 ctx (*inp*)src src key;
+    Poly1305.Equiv.lemma_poly1305_equiv src key;
+    assert (B.as_seq h1 dst == Spec.Poly1305.poly1305 (B.as_seq h0 src) (B.as_seq h0 key));
     pop_frame ()
   end else begin
     Hacl.Poly1305_32.poly1305_mac dst src len key;
